# Checking Implication

Checking implication is an important step for proving one-path and all-path reachability claims.
This document will describe logically how this step will be performed.

## Background

The reader should be familiar with the algorithm for proving one-path and all-path reachability claims:

- [One-Path](2018-11-08-One-Path-Reachability-Proofs.md)
- [All-Path](2019-03-28-All-Path-Reachability-Proofs.md)

## Problem

Consider a reachability claim,

```
φ(X) → ∘ ∃ Y. ψ(X, Y)
```

where `∘` denotes the appropriate one-path or all-path modality
and `X` and `Y` denote _distinct_ families of variables.
We will assume that `φ(X)` and `ψ(X, Y)` are function-like patterns (matching at most one value)
because this is true in typical use.

The reachability proof algorithm will unroll the modality, giving

```
φ(X) → ∃ Y. ψ(X, Y) ∨ • ∘ ∃ Y. ψ(X, Y)
===
φ(X) ∧ ¬ ∃ Y. ψ(X, Y) → • ∘ ∃ Y. ψ(X, Y)
```

If the direct implication holds, then

```
φ(X) ∧ ¬ ∃ Y. ψ(X, Y)
```

is unsatisfiable.
Otherwise, the reachability proof algorithm continues by rewriting the configuration.

## Solution

Checking that the formula

```
φ(X) ∧ ¬ ∃ Y. ψ(X, Y)
```

is unsatisfiable is equivalent to checking

```
⌈φ(X) ∧ ¬ ∃ Y. ψ(X, Y)⌉.
```

Because we assume that `φ(X)` is a function-like pattern,
we can move the negation outside of `⌈ ⌉`:

```
⌈φ(X) ∧ ¬ ∃ Y. ψ(X, Y)⌉
===
¬ ⌈φ(X) ∧ ∃ Y. ψ(X, Y)⌉ ∧ ⌈φ(X)⌉.
```

By alpha-equivalence, we can also move the quantifier outside of `⌈ ⌉`:

```
(¬ ⌈φ(X) ∧ ∃ Y. ψ(X, Y)⌉) ∧ ⌈φ(X)⌉
===
(¬ ∃ Y. ⌈φ(X) ∧ ψ(X, Y)⌉) ∧ ⌈φ(X)⌉.
```

## Optimization

We can optimize this solution in the typical case where

```
φ(X) = t(X) ∧ P(X)
ψ(X, Y) = ⋁ᵢ tᵢ(X, Y) ∧ Pᵢ(X, Y)
```

where `t(X)` and `tᵢ(X, Y)` are term-like patterns
and `P(X)` and `Pᵢ(X, Y)` are predicates.
The unification of the left- and right-hand sides is

```
∃ Y. ⌈φ(X) ∧ ψ(X, Y)⌉
===
⋁ᵢ ∃ Y. ⌈t(X) ∧ tᵢ(X, Y)⌉ ∧ P(X) ∧ Pᵢ(X, Y)
===
P(X) ∧ ⋁ᵢ ∃ Y. ⌈t(X) ∧ tᵢ(X, Y)⌉ ∧ Pᵢ(X, Y)
```

so that

```
(¬ ∃ Y. ⌈φ(X) ∧ ψ(X, Y)⌉) ∧ ⌈φ(X)⌉
===
  ¬ P(X) ∧ ⌈φ(X)⌉
∨
  (¬ ⋁ᵢ ∃ Y. ⌈t(X) ∧ tᵢ(X, Y)⌉ ∧ Pᵢ(X, Y)) ∧ ⌈φ(X)⌉
```

The first term of the above disjuntion is `⊥`,

```
¬ P(X) ∧ ⌈φ(X)⌉
===
¬ P(X) ∧ ⌈t(X)⌉ ∧ P(X)
===
⊥
```

leaving only

```
(¬    ∃ Y. ⌈φ(X) ∧ ψ(X, Y)⌉            ) ∧ ⌈φ(X)⌉
===
(¬ ⋁ᵢ ∃ Y. ⌈t(X) ∧ tᵢ(X, Y)⌉ ∧ Pᵢ(X, Y)) ∧ ⌈t(X)⌉ ∧ P(X).
===
(⋀ᵢ ¬ ∃ Y. ⌈t(X) ∧ tᵢ(X, Y)⌉ ∧ Pᵢ(X, Y)) ∧ ⌈t(X)⌉ ∧ P(X).
```

The sub-terms `⌈t(X) ∧ tᵢ(X, Y)⌉` are unification problems with an efficient internal implementation.
The unification problems should be solved first because

```
⌈t(X) ∧ tᵢ(X, Y)⌉ → ⌈t(X)⌉
```

so that if unification succeeds on any branch, there is no need to explicitly consider `⌈t(X)⌉`.
If unification fails, then the negative conjunct is `\top` so that the implication is satisified only when `⌈t(X)⌉ ∧ P(X)` is unsatisfiable.
Now, the implication is checked in two cases:
after a configuration is rewritten (in which case the configuration may be rewritten again)
or after a configuration can no longer be rewritten (a remainder pattern).
In the case of a rewritten configuration, when unification fails, there is no need to check the rest of the implication pattern:
the condition `t(X) ∧ P(X)` itself implies the condition `⌈t(X)⌉ ∧ P(X)`.

## Summary

The algorithm follows:

Given the implication

```
φ(X) → ∃ Y. ψ(X, Y)
```

with

```
φ(X) = t(X) ∧ P(X)
ψ(X, Y) = ⋁ᵢ tᵢ(X, Y) ∧ Pᵢ(X, Y)
```

where `t(X)` and `tᵢ(X, Y)` are term-like patterns
and `P(X)` and `Pᵢ(X, Y)` are predicates,

1. Solve the unification problems `⌈t(X) ∧ tᵢ(X, Y)⌉`.
2. If unification succeeds on any branch, evaluate
   `(⋀ᵢ ¬ ∃ Y. ⌈t(X) ∧ tᵢ(X, Y)⌉ ∧ Pᵢ(X, Y)) ∧ ⌈t(X)⌉ ∧ P(X)`.
   1. If the predicate is unsatisfiable,
      then the implication is valid.
   2. If the predicate is satisfiable,
      conjoin it with the configuration and continue rewriting.
      (Note: At the time of writing,
      the backend does not conjoin the predicate with the configuration.
      This is sound, but not complete.)
3. If unification fails on all branches,
   1. If `φ(X)` is a remainder pattern, evaluate
      `⌈t(X)⌉ ∧ P(X)`.
      The implication is valid iff the predicate is unsatisfiable.
   2. If `φ(X)` is a rewritten pattern, assume the implication is not valid.
      (Aside: If we checked `⌈t(X)⌉ ∧ P(X)` here,
      then we could infer that the configuration is defined,
      allowing us to do subsequent rewriting without generating extra definedness conditions.
      The efficiency of this method merits investigation.)
